Soundness

stlc/soundness.v
@@ -1,22 +1,49 @@
 From stlc Require Export fundamental.
 From iris.proofmode Require Import tactics.
 From iris.program_logic Require Import adequacy.
+From iris.base_logic Require Export gen_heap.
 
-Lemma wp_soundness `{irisG stlc_lang Σ} e τ : [] ⊢ₜ e : τ → ⊢ WP e {{ ⟦ τ ⟧ }}.
-Proof.
-  iIntros (?).
-  replace e with e.[env_subst[]] by by asimpl.
-  iApply fundamental; eauto. iApply interp_env_nil.
-Qed.
+Definition log_typed `{irisG stlc_lang Σ} (Γ : list type) (e : expr stlc_lang) (τ : type) := ∀ Δ vs,
+  env_Persistent Δ →
+  ⟦ Γ ⟧* Δ vs ⊢ ⟦ τ ⟧ₑ Δ e.[env_subst vs].
+Notation "Γ ⊨ e : τ" := (log_typed Γ e τ) (at level 74, e, τ at next level).
 
-Theorem soundness e τ e' thp :
-  [] ⊢ₜ e : τ → rtc erased_step ([e], ()) (thp, ()) → e' ∈ thp → not_stuck e' ().
+Class stlcPreIG Σ := HeapPreIG {
+  stlc_preG_iris :> invPreG Σ;
+  stlc_preG_heap :> gen_heapPreG () (val stlc_lang) Σ
+}.
+
+Theorem soundness Σ `{stlcPreIG Σ} e τ e' thp σ σ' :
+  (∀ `{irisG stlc_lang Σ}, [] ⊨ e : τ) →
+  rtc erased_step ([e], σ) (thp, σ') → e' ∈ thp →
+  not_stuck e' σ'.
 Proof.
-  set (Σ := invΣ). intros.
-  cut (adequate NotStuck e () (λ _ _, True));
+  intros Hlog ??.
+  cut (adequate NotStuck e σ (λ _ _, True));
     first by intros [_ Hsafe]; eapply Hsafe; eauto.
   eapply (wp_adequacy Σ _). iIntros (Hinv ?).
-  iModIntro. iExists (λ _ _, True%I), (λ _, True%I). iSplit=>//.
-  set (HΣ := IrisG _ _ Hinv (λ _ _ _ _, True)%I (λ _, True)%I).
-  iApply (wp_wand with "[]"). by iApply wp_soundness. eauto.
+  destruct H.
+  red in σ.
+  iMod (gen_heap_init empty) as (Hheap) "[Hh _]".
+  iModIntro.
+  iExists (λ σ _, gen_heap_interp empty), (λ _, True%I); iFrame.
+  (* set (HeapΣ := (irisG stlc_lang Σ)). *)
+  iApply (wp_wand with "[]").
+  - replace e with e.[env_subst[]] by by asimpl.
+    iApply (Hlog _ [] []). iApply (@interp_env_nil _ _).
+  - eauto.
 Qed.
+
+Corollary type_soundness e τ e' thp σ σ' :
+  [] ⊢ₜ e : τ →
+  rtc erased_step ([e], σ) (thp, σ') → e' ∈ thp → not_stuck e' σ'.
+Proof.
+  intros ??.
+  set (Σ := #[invΣ ; gen_heapΣ () (val stlc_lang)]).
+  set (HG := HeapPreIG Σ _ _).
+  eapply (soundness Σ); eauto using fundamental.
+  Unshelve. 2 : exact τ. intros.
+  eapply fundamental. eauto.
+Qed.
+
+
