stlc/rules.v
@@ -30,9 +30,7 @@ Section stlc_rules.
     intros ?; apply nsteps_once, pure_head_step_pure_step;
       constructor; [solve_exec_safe | solve_exec_puredet].
 
-
   (** Helper Lemmas for weakestpre. *)
-
   Global Instance pure_rec e1 e2 `{!AsVal e2} :
       PureExec True 1 (App (Rec e1) e2) e1.[(Rec e1), e2 /].
   Proof. solve_pure_exec. Qed.
@@ -59,8 +57,5 @@ Section stlc_rules.
   Global Instance pure_case_inr e0 e1 e2 `{!AsVal e0}:
     PureExec True 1 (Case (InjR e0) e1 e2) e2.[e0/].
   Proof. solve_pure_exec. Qed.
-
-
-
 
 End stlc_rules.
